working on linker

assembler/RelocProgLinking.v
@@ -5,11 +5,104 @@ Import ListNotations.
 
 Local Open Scope list_scope.
 
-Definition link_reloc_prog (F V I D: Type) (p1 p2: program F V I D) : option (program F V I D) := None.
+Definition link_symbentry (e1 e2 : symbentry) :=
+  match e1.(symbentry_bind),e2.(symbentry_bind) with
+  | bind_local,_ => None
+  | _,bind_local => None
+  | _,_ => match e1.(symbentry_secindex),e2.(symbentry_secindex) with
+          | secindex_normal _, secindex_undef => Some e1
+          | secindex_undef, secindex_normal _ => Some e2
+          | secindex_comm, secindex_undef => Some e1
+          | secindex_undef, secindex_comm => Some e2
+          | secindex_undef,secindex_undef => Some e1
+          | _,_ => None
+          end
+  end.
 
-Program Instance Linker_reloc_prog (F V I D : Type) : Linker (program F V I D) :=
-{
-  link := (link_reloc_prog F V I D);
-  linkorder := fun _ _ => True;
-}.
+Inductive linkorder_symbentry: symbentry -> symbentry -> Prop :=
+| linkorder_symbentry_refl: forall e, linkorder_symbentry e e
+| linkorder_symbentry_undef_any:
+  forall e1 e2, e1.(symbentry_secindex) = secindex_undef ->
+           linkorder_symbentry e1 e2.
 
+Program Instance Linker_symbentry : Linker symbentry := {
+    link:= link_symbentry;
+    linkorder:= linkorder_symbentry
+  }.
+Next Obligation.
+  constructor.
+Defined.
+Next Obligation.
+  inv H;inv H0;try constructor;auto.
+Defined.
+Next Obligation.
+  unfold link_symbentry in H.
+  repeat destr_in H;
+  split;try constructor;auto.
+Defined.
+
+Global Opaque Linker_symbentry.
+
+Definition check_symbentry (e1 e2 : symbentry) :=
+  match e1.(symbentry_bind),e2.(symbentry_bind) with
+  | bind_local,_ => false
+  | _,bind_local => false
+  | _,_ => match e1.(symbentry_secindex),e2.(symbentry_secindex) with
+          | secindex_normal _, secindex_undef => true
+          | secindex_undef, secindex_normal _ => true
+          | secindex_comm, secindex_undef =>     true
+          | secindex_undef, secindex_comm =>     true
+          | secindex_undef,secindex_undef =>     true
+          | _,_ => false
+          end
+  end.
+
+Definition link_section_merge {I D:Type} (o1 o2 : option (section I D)) :=
+  match o1,o2 with
+  | None,_ => o2
+  | _,None => o1
+  | Some e1,Some e2 => None
+  end.
+
+Definition link_reloctable_merge (o1 o2 : option reloctable) :=
+  match o1,o2 with
+  | None,_ => o2
+  | _,None => o1
+  | Some e1,Some e2 => None
+  end.
+
+
+Section LINKER_PROG.
+
+Context {F V I D: Type} {LF: Linker F} {LV: Linker V} (p1 p2: program F V I D).
+
+Definition link_relocprog_check (x:ident) (e1: symbentry) :=
+  match p2.(prog_symbtable)!x with
+  | Some e2 => check_symbentry e1 e2
+  | _ => true
+  end.
+      
+
+Definition link_reloc_prog :=
+  let ap1 := 
+      {| AST.prog_defs   := prog_defs p1;
+         AST.prog_public := prog_public p1;
+         AST.prog_main   := prog_main p1; |} in
+  let ap2 := 
+      {| AST.prog_defs   := prog_defs p2;
+         AST.prog_public := prog_public p2;
+        AST.prog_main   := prog_main p2; |} in
+  match link ap1 ap2 with
+  | None => None
+  | Some ap =>
+      if PTree_Properties.for_all p1.(prog_symbtable) link_relocprog_check then
+        Some {| prog_defs := PTree.elements (PTree.combine link_prog_merge (PTree_Properties.of_list p1.(prog_defs)) (PTree_Properties.of_list p2.(prog_defs)));
+               prog_public := p1.(prog_public) ++ p2.(prog_public);    
+               prog_main := p1.(prog_main);           
+               prog_sectable := PTree.combine link_section_merge p1.(prog_sectable) p2.(prog_sectable);
+               prog_symbtable := PTree.combine link p1.(prog_symbtable) p2.(prog_symbtable);
+               prog_reloctables := PTree.combine link_reloctable_merge p1.(prog_reloctables) p2.(prog_reloctables);
+               prog_senv := Globalenvs.Genv.to_senv (Globalenvs.Genv.globalenv ap); |}
+      else None
+    end.
+    
